coqimp/framework/soundness/inssound.v
@@ -5,13 +5,13 @@ Require Import LibTactics.
 Require Import Integers. 
 Open Scope Z_scope.  
 Import ListNotations. 
-
+ 
 Set Asymmetric Patterns.
    
 Require Import state. 
 Require Import language.
 
-Set Implicit Arguments.
+Set Implicit Arguments. 
 Unset Strict Implicit.
       
 Require Import logic. 
@@ -23,6 +23,8 @@ Require Import Coq.Logic.FunctionalExtensionality.
 
 Open Scope nat.
 Open Scope code_scope.
+
+(*+ Auxiliary Definition +*)
 
 (*+ Lemmas for Memory Model +*)
 Lemma memset_l_l_indom :
@@ -326,6 +328,107 @@ Proof.
   }
 Qed.
 
+Lemma indom_dom_eq_subst :
+  forall tp l (m m' : tp -> option Word),
+    indom l m ->
+    dom_eq m m' ->
+    indom l m'.
+Proof.
+  intros.
+  unfold dom_eq in *.
+  simpljoin1.
+  eauto.
+Qed.
+
+Lemma indom_dom_eq_merge_subst :
+  forall tp l (m1 m1' m2 : tp -> option Word),
+    indom l (merge m1 m2) ->
+    dom_eq m1 m1' ->
+    indom l (merge m1' m2).
+Proof.
+  intros.
+  unfold indom in *.
+  unfold dom_eq in *.
+  simpljoin1.
+  unfold merge in *.
+  destruct (m1 l) eqn:Heqe1.
+  {
+    assert (indom l m1).
+    unfold indom; eauto.
+    eapply H0 in H2; eauto.
+    unfold indom in *.
+    simpljoin1; eauto.
+    eexists.
+    rewrite H2; eauto.
+  }
+  {
+    destruct (m1' l) eqn:Heqe2; eauto.
+  }
+Qed.
+
+Lemma indom_dom_eq_merge_subst2 :
+  forall tp l (m1 m2 m2' : tp -> option Word),
+    indom l (merge m1 m2) ->
+    dom_eq m2 m2' ->
+    indom l (merge m1 m2').
+Proof.
+  intros.
+  unfold indom in *.
+  unfold dom_eq in *.
+  simpljoin1.
+  unfold merge in *. 
+  destruct (m1 l) eqn:Heqe1.
+  {
+    inversion H; eauto.
+  }
+  {
+    assert (indom l m2).
+    unfold indom; eauto.
+    eapply H0 in H2; eauto.
+  }
+Qed.
+
+Lemma dom_eq_merge_subst1 :
+  forall tp (m m' m1 m2 : tp -> option Word),
+    dom_eq m m' ->
+    dom_eq (merge m m1) m2 ->
+    dom_eq (merge m' m1) m2.
+Proof.
+  intros.
+  unfold dom_eq in *.
+  split.
+  {
+    intros.
+    simpljoin1.
+    eapply H0.
+    eapply indom_dom_eq_merge_subst; eauto.
+    unfold dom_eq; eauto.
+  }
+  {
+    simpljoin1.
+    intros.
+    eapply H1 in H3.
+    eapply indom_dom_eq_merge_subst; eauto.
+    unfold dom_eq; eauto.
+  }
+Qed.
+
+Lemma dom_eq_sym :
+  forall tp (m m' : tp -> option Word),
+    dom_eq m m' -> dom_eq m' m.
+Proof.
+  intros.
+  unfold dom_eq in *.
+  simpljoin1.
+  split.
+  {
+    intros; eauto.
+  }
+  {
+    intros; eauto.
+  }
+Qed.
+
 Lemma disj_in_m1_merge_still :
   forall tp (m1 m2 : tp -> option Word) l v,
     disjoint m1 m2 -> m1 l = Some v ->
@@ -355,7 +458,57 @@ Proof.
   }
 Qed.
 
+(*+ Lemmas for expression +*)
+Lemma eval_opexp_merge_still2 :
+  forall R r oexp l,
+    eval_opexp r oexp = Some l -> disjoint R r ->
+    eval_opexp (merge R r) oexp = Some l.
+Proof.
+  intros.
+  destruct oexp.
+  {
+    simpls. 
+    eapply get_vl_merge_still2; eauto.
+  }
+  {
+    simpls.
+    eauto.
+  }
+Qed.
+
 (*+ Lemmas for Register State +*)
+Lemma indom_setR_still :
+  forall l rn R v,
+    indom l R ->
+    indom l (set_R R rn v).
+Proof.
+  intros.
+  unfold indom in *.
+  simpljoin1.
+  unfold set_R in *.
+  unfold is_indom in *.
+  destruct (R rn) eqn:Heqe.
+  {
+    unfolds RegMap.set.
+    destruct_rneq.
+  }
+  {
+    eauto.
+  }
+Qed.
+
+Lemma indom_regset_still:
+  forall l l' M w,
+    indom l M ->
+    indom l (RegMap.set l' (Some w) M).
+Proof.
+  intros.
+  unfold indom in *.
+  simpljoin1.
+  unfold RegMap.set.
+  destruct_rneq.
+Qed.
+
 Lemma RegSet_same_addr_disj_stable2 :
   forall l v v' m m',
     disjoint m (RegMap.set l (Some v') m') ->
@@ -678,6 +831,25 @@ Proof.
   }
 Qed.
 
+Lemma rn_st_v_eval_reg_v :
+  forall M R F D rn w p,
+    (M, (R, F), D) |= rn |=> w ** p ->
+    R rn = Some w.
+Proof.
+  intros.
+  simpls.
+  simpljoin1.
+  destruct_state x.
+  destruct_state x0.
+  simpls.
+  simpljoin1.
+  unfolds regSt.
+  simpls; simpljoin1.
+  unfold merge.
+  unfold RegMap.set.
+  destruct_rneq.
+Qed.
+
 Ltac disj_reg_solve :=
   match goal with
   | H : disjoint (RegMap.set ?l1 (Some ?v1) empR)
@@ -854,6 +1026,184 @@ Proof.
   }
 Qed.
 
+Lemma indoms_merge_still1 :
+  forall tp vl (m1 m2 : tp -> option Word),
+    indoms vl m1 ->
+    indoms vl (merge m1 m2).
+Proof.
+  intros tp vl.
+  induction vl; intros.
+  -
+    simpl; eauto.
+
+  -
+    simpl in H.
+    simpljoin1.
+    simpl. 
+    split; eauto.
+    eapply indom_merge_still; eauto.
+Qed.
+
+Lemma indoms_merge_still2 :
+  forall tp vl (m1 m2 : tp -> option Word),
+    indoms vl m2 ->
+    indoms vl (merge m1 m2).
+Proof.
+  intros tp vl.
+  induction vl; intros.
+  -
+    simpl; eauto.
+
+  -
+    simpl in H.
+    simpljoin1.
+    simpl.
+    split; eauto.
+    eapply indom_merge_still2; eauto.
+Qed.
+
+Lemma indoms_setR_still :
+  forall vl R rn w, 
+    indoms (getRs vl) R ->
+    indoms (getRs vl) (set_R R rn w).
+Proof.
+  intro vl.
+  induction vl; intros.
+  -
+    simpls.
+    eauto.
+  -
+    destruct a.
+    simpls.
+    simpljoin1.
+    split.
+    eapply indom_setR_still; eauto.
+    eauto.
+Qed.
+
+Lemma indoms_setRs_merge_eq :
+  forall vl R r,
+    indoms (getRs vl) R ->
+    set_Rs (merge R r) vl = merge (set_Rs R vl) r.
+Proof.
+  intros vl.
+  induction vl; intros.
+  -
+    simpls.
+    eauto.
+  -
+    destruct a.
+    simpl in H.
+    simpl. 
+    simpljoin1.
+    rewrite indom_setR_merge_eq1; eauto.
+    eapply IHvl.
+    eapply indoms_setR_still; eauto.
+Qed.
+
+Lemma indoms_setRs_merge_eq2 :
+  forall vl (R : RegFile) r,
+    disjoint R r ->
+    indoms (getRs vl) r ->
+    set_Rs (merge R r) vl = merge R (set_Rs r vl).
+Proof.
+  intros vl.
+  induction vl; intros.
+  -
+    simpls.
+    eauto.
+  -
+    destruct a.
+    simpl in H0.
+    simpl.
+    simpljoin1.
+     
+    rewrite indom_setR_merge_eq2; eauto.
+    eapply IHvl.
+    eapply disjoint_setR_still2; eauto.
+    eapply indoms_setR_still; eauto.
+    clear - H H0.
+    intro.
+    unfold disjoint in *.
+    specialize (H r0).
+    unfold indom in *.
+    simpljoin1.
+    rewrite H1 in H; eauto.
+    rewrite H0 in H; eauto.
+Qed.
+
+Lemma Reg_upd :
+  forall M R F D rn w w' p,
+    (M, (R, F), D) |= rn |=> w ** p ->
+    (M, (RegMap.set rn (Some w') R, F), D) |= rn |=> w' ** p.
+Proof.
+  intros.
+  simpl in H.
+  simpljoin1.
+  destruct_state x.
+  destruct_state x0.
+  simpl in H.
+  simpljoin1.
+  unfolds regSt.
+  simpls.
+  simpljoin1.
+  exists (empM, (RegMap.set rn (Some w') empR, f0), d0) (m0, (r0, f0), d0).
+  repeat (split; eauto).
+  eapply RegSet_same_addr_disj_stable; eauto.
+
+  rewrite indom_setR_merge_eq; eauto.
+  rewrite regset_twice; eauto.
+  eapply regset_l_l_indom; eauto.
+Qed.
+
+Definition precise_asrt (p : asrt) :=
+  forall M M' R R' F D,
+    (M, (R, F), D) |= p -> (M', (R', F), D) |= p ->
+    M = M' /\ R = R'.
+
+Lemma regst_precise :
+  forall rn w,
+    precise_asrt (rn |=> w).
+Proof.   
+  unfold precise_asrt.
+  intros.
+  simpls.
+  unfolds regSt.
+  simpls.
+  simpljoin1.
+  eauto.
+Qed.
+
+Lemma precise_star :
+  forall p1 p2,
+    precise_asrt p1 -> precise_asrt p2 ->
+    precise_asrt (p1 ** p2).
+Proof. 
+  intros.
+  unfolds precise_asrt.
+  intros.
+  sep_star_split_tac.
+  simpl in H4, H6.
+  simpljoin1.
+  eapply H in H1; eauto.
+  eapply H0 in H3; eauto.
+  subst.
+  eauto.
+  simpljoin1.
+  subst.
+  eauto.
+Qed.
+
+Lemma Reg_frm_precise :
+  forall (rr0 rr1 rr2 rr3 rr4 rr5 rr6 rr7 : GenReg) w0 w1 w2 w3 w4 w5 w6 w7,
+    precise_asrt (rr0 |=> w0 ** rr1 |=> w1 ** rr2 |=> w2 ** rr3 |=> w3 **
+                      rr4 |=> w4 ** rr5 |=> w5 ** rr6 |=> w6 ** rr7 |=> w7).
+Proof.
+  intros.
+  repeat (eapply precise_star; [eapply regst_precise | idtac]).
+  eapply regst_precise; eauto.
+Qed.
+
 (*+ Lemmas for Frame List +*)
 Lemma frame_asrt_upd :
   forall M R D id id' F F',
@@ -965,9 +1315,54 @@ Lemma reg_st_fetch_frame :
     Some ([[w0, w1, w2, w3, w4, w5, w6, w7]]).
 Proof.
   intros.
-
-  >>>>>>>>>>>>>>>>>>>>>>>>>
   unfold fetch_frame.
+
+  assert (R rr0 = Some w0).
+  {
+    eapply rn_st_v_eval_reg_v; eauto.
+  }
+  assert (R rr1 = Some w1).
+  {
+    eapply sep_star_lift in H.
+    eapply rn_st_v_eval_reg_v; eauto.
+  }
+  assert (R rr2 = Some w2).
+  {
+    eapply sep_star_assoc in H.
+    eapply sep_star_lift in H.
+    eapply rn_st_v_eval_reg_v; eauto.
+  }
+  assert (R rr3 = Some w3).
+  {
+    do 2 eapply sep_star_assoc in H.
+    eapply sep_star_lift in H.
+    eapply rn_st_v_eval_reg_v; eauto.
+  }
+  assert (R rr4 = Some w4).
+  {
+    do 3 eapply sep_star_assoc in H.
+    eapply sep_star_lift in H.
+    eapply rn_st_v_eval_reg_v; eauto.
+  }
+  assert (R rr5 = Some w5).
+  {
+    do 4 eapply sep_star_assoc in H.
+    eapply sep_star_lift in H.
+    eapply rn_st_v_eval_reg_v; eauto.
+  }
+  assert (R rr6 = Some w6).
+  {
+    do 5 eapply sep_star_assoc in H.
+    eapply sep_star_lift in H.
+    eapply rn_st_v_eval_reg_v; eauto.
+  }
+  assert (R rr7 = Some w7).
+  {
+    do 6 eapply sep_star_assoc in H.
+    eapply sep_star_sym in H.
+    eapply rn_st_v_eval_reg_v in H; eauto.
+  }
+  
   rewrite H0; eauto.
   rewrite H1; eauto.
   rewrite H2; eauto.
@@ -1026,6 +1421,65 @@ Proof.
   eauto.
 Qed.
 
+Ltac eval_reg_merge_solve1 :=
+  match goal with
+  | H : context [?R ?rn] |- context [(merge ?R ?R') ?rn] =>
+    let Heqe := fresh in
+    destruct (R rn) eqn:Heqe;
+    [ eapply get_vl_merge_still in Heqe; eauto;
+      try rewrite Heqe; eval_reg_merge_solve1 | tryfalse]
+  | _ => idtac
+  end.
+
+Ltac eval_reg_merge_solve2 :=
+  match goal with
+  | H : context [?R ?rn] |- context [(merge ?R' ?R) ?rn] =>
+    let Heqe := fresh in
+    destruct (R rn) eqn:Heqe;
+    [ eapply get_vl_merge_still2 in Heqe; eauto;
+      try rewrite Heqe; eval_reg_merge_solve2 | tryfalse]
+  | _ => idtac
+  end.
+
+Lemma fetch_frame_disj_merge_stable1 :
+  forall R1 R2 rr0 rr1 rr2 rr3 rr4 rr5 rr6 rr7 fm,
+    disjoint R1 R2 ->
+    fetch_frame R1 rr0 rr1 rr2 rr3 rr4 rr5 rr6 rr7 = Some fm ->
+    fetch_frame (merge R1 R2) rr0 rr1 rr2 rr3 rr4 rr5 rr6 rr7 = Some fm.
+Proof.
+  intros.
+  unfolds fetch_frame.
+
+  eval_reg_merge_solve1.
+  eauto.
+Qed.
+
+Lemma fetch_frame_disj_merge_stable2 :
+  forall R1 R2 rr0 rr1 rr2 rr3 rr4 rr5 rr6 rr7 fm,
+    disjoint R1 R2 ->
+    fetch_frame R2 rr0 rr1 rr2 rr3 rr4 rr5 rr6 rr7 = Some fm ->
+    fetch_frame (merge R1 R2) rr0 rr1 rr2 rr3 rr4 rr5 rr6 rr7 = Some fm.
+Proof.
+  intros.
+  unfolds fetch_frame.
+
+  eval_reg_merge_solve2.
+  eauto.
+Qed.
+
+Lemma disjoint_setfrm_still :
+  forall R r rr0 rr1 rr2 rr3 rr4 rr5 rr6 rr7 fm,
+    disjoint R r ->
+    disjoint (set_frame R rr0 rr1 rr2 rr3 rr4 rr5 rr6 rr7 fm) r.
+Proof. 
+  intros.
+  unfold set_frame.
+  destruct fm.
+  simpl.
+  >>>>>>>>>>>>>>>>>>>>>>>>
+  repeat (eapply disjoint_setR_still; eauto).
+Qed.
+
 Lemma fetch_disj_merge_still1 :
   forall R R1 fms,
     fetch R = Some fms ->
@@ -1078,7 +1532,7 @@ Qed.
 Lemma LocalRegs_fetch :
   forall M R F D fm,
     (M, (R, F), D) |= LocalRegs fm ->
-    fetch_frame M R r16 r17 r18 r19 r20 r21 r22 r23 = Some fm.
+    fetch_frame R r16 r17 r18 r19 r20 r21 r22 r23 = Some fm.
 Proof.
   intros.
   unfolds LocalRegs.
@@ -1089,7 +1543,7 @@ Qed.
 Lemma InRegs_fetch :
   forall M R F D fm,
     (M, (R, F), D) |= InRegs fm ->
-    fetch_frame M R r24 r25 r26 r27 r28 r29 r30 r31 = Some fm.
+    fetch_frame R r24 r25 r26 r27 r28 r29 r30 r31 = Some fm.
 Proof.
   intros.
   unfolds InRegs.
@@ -1100,7 +1554,7 @@ Qed.
 Lemma Regs_fetch :
   forall M R F D fm1 fm2 fm3,
     (M, (R, F), D) |= Regs fm1 fm2 fm3 ->
-    fetch M R = Some [fm1; fm2; fm3].
+    fetch R = Some [fm1; fm2; fm3].
 Proof.
   intros.
   unfolds Regs.
@@ -1122,18 +1576,538 @@ Proof.
 
   unfold fetch.
 
-  eapply fetch_frame_disj_merge_stable1 with (m2 := merge m1 m2) in H; eauto.
+  eapply fetch_frame_disj_merge_stable1 with (R2 := merge r1 r2) in H; eauto.
   rewrite H.
 
-  eapply fetch_frame_disj_merge_stable1 with (m2 := m2) in H0; eauto.
+  eapply fetch_frame_disj_merge_stable1 with (R2 := r2) in H0; eauto.
   eapply fetch_frame_disj_merge_stable2 in H0; eauto.
   rewrite H0; eauto.
 
-  eapply fetch_frame_disj_merge_stable2 with (m1 := m1) in H2; eauto.
-  eapply fetch_frame_disj_merge_stable2 with (m1 := m) in H2; eauto.
+  eapply fetch_frame_disj_merge_stable2 with (R1 := r1) in H2; eauto.
+  eapply fetch_frame_disj_merge_stable2 with (R1 := r) in H2; eauto.
 
   rewrite H2; eauto.
 Qed.
+
+Lemma indom_setfrm_still :
+  forall l R fm rr0 rr1 rr2 rr3 rr4 rr5 rr6 rr7,
+    indom l R ->
+    indom l (set_frame R rr0 rr1 rr2 rr3 rr4 rr5 rr6 rr7 fm).
+Proof.
+  intros.
+  unfold set_frame.
+  destruct fm; eauto.
+  simpl.
+  repeat (eapply indom_setR_still); eauto.
+Qed.
+  
+Lemma indom_setwin_still :
+  forall l R fm1 fm2 fm3,
+    indom l R ->
+    indom l (set_window R fm1 fm2 fm3).
+Proof.
+  intros.
+  unfold set_window.
+  repeat (eapply indom_setfrm_still; eauto).
+Qed.
+
+Lemma indoms_set_frm_still :
+  forall (vl : list GenReg) (R : RegFile) fm (rr0 rr1 rr2 rr3 rr4 rr5 rr6 rr7 : GenReg),
+    indoms vl R ->
+    indoms vl (set_frame R rr0 rr1 rr2 rr3 rr4 rr5 rr6 rr7 fm).
+Proof.
+  intro vl.
+  induction vl; intros.
+  -
+    simpls. eauto.
+  -
+    simpls.
+    simpljoin1.
+    split.
+    eapply indom_setfrm_still; eauto.
+    eauto.
+Qed.
+
+Lemma regfrm_indoms :
+  forall M R F D (rr0 rr1 rr2 rr3 rr4 rr5 rr6 rr7 : GenReg)
+    (w0 w1 w2 w3 w4 w5 w6 w7 : Word),
+    (M, (R, F), D) |=
+                   rr0 |=> w0 ** rr1 |=> w1 ** rr2 |=> w2 ** rr3 |=> w3 **
+                   rr4 |=> w4 ** rr5 |=> w5 ** rr6 |=> w6 ** rr7 |=> w7 ->
+    indoms [rr0; rr1; rr2; rr3; rr4; rr5; rr6; rr7] R.
+Proof.
+  intros.
+  simpl.
+  
+  split.
+  eapply rn_st_v_eval_reg_v in H.
+  unfold indom; eauto.
+
+  split.
+  eapply sep_star_lift in H.
+  eapply rn_st_v_eval_reg_v in H.
+  unfold indom; eauto.
+
+  split.
+  eapply sep_star_assoc in H.
+  eapply sep_star_lift in H.
+  eapply rn_st_v_eval_reg_v in H.
+  unfold indom; eauto.
+
+  split.
+  do 2 eapply sep_star_assoc in H.
+  eapply sep_star_lift in H.
+  eapply rn_st_v_eval_reg_v in H.
+  unfold indom; eauto.
+
+  split.
+  do 3 eapply sep_star_assoc in H.
+  eapply sep_star_lift in H.
+  eapply rn_st_v_eval_reg_v in H.
+  unfold indom; eauto.
+
+  split.
+  do 4 eapply sep_star_assoc in H.
+  eapply sep_star_lift in H.
+  eapply rn_st_v_eval_reg_v in H.
+  unfold indom; eauto.
+
+  split.
+  do 5 eapply sep_star_assoc in H.
+  eapply sep_star_lift in H.
+  eapply rn_st_v_eval_reg_v in H.
+  unfold indom; eauto.
+
+  split.
+  do 6 eapply sep_star_assoc in H.
+  eapply sep_star_sym in H.
+  eapply rn_st_v_eval_reg_v in H.
+  unfold indom; eauto.
+
+  eauto.
+Qed.
+
+Lemma OutRegs_indoms :
+  forall M R F D fm,
+    (M, (R, F), D) |= OutRegs fm ->
+    indoms [r8; r9; r10; r11; r12; r13; r14; r15] R.
+Proof.
+  intros.
+  unfolds OutRegs.
+  destruct fm.
+  eapply regfrm_indoms; eauto.
+Qed.
+
+Lemma LocalRegs_indoms :
+  forall M R F D fm,
+    (M, (R, F), D) |= LocalRegs fm ->
+    indoms [r16; r17; r18; r19; r20; r21; r22; r23] R.
+Proof.
+  intros.
+  unfolds LocalRegs.
+  destruct fm.
+  eapply regfrm_indoms; eauto.
+Qed.
+
+Lemma InRegs_indoms :
+  forall M R F D fm,
+    (M, (R, F), D) |= InRegs fm ->
+    indoms [r24; r25; r26; r27; r28; r29; r30; r31] R.
+Proof.
+  intros.
+  unfolds InRegs.
+  destruct fm.
+  eapply regfrm_indoms; eauto.
+Qed.
+
+Lemma fetch_some_set_frm_merge_eq :
+  forall (R r : RegFile) fm (rr0 rr1 rr2 rr3 rr4 rr5 rr6 rr7 : GenReg),
+    indoms [rr0; rr1; rr2; rr3; rr4; rr5; rr6; rr7] R ->
+    set_frame (merge R r) rr0 rr1 rr2 rr3 rr4 rr5 rr6 rr7 fm =
+    merge (set_frame R rr0 rr1 rr2 rr3 rr4 rr5 rr6 rr7 fm) r.
+Proof.
+  intros.
+  unfolds set_frame.
+  destruct fm.
+  eapply indoms_setRs_merge_eq; eauto.
+Qed.
+
+Lemma fetch_some_set_frm_merge_eq2 :
+  forall (R r : RegFile) fm (rr0 rr1 rr2 rr3 rr4 rr5 rr6 rr7 : GenReg),
+    disjoint R r ->
+    indoms [rr0; rr1; rr2; rr3; rr4; rr5; rr6; rr7] r ->
+    set_frame (merge R r) rr0 rr1 rr2 rr3 rr4 rr5 rr6 rr7 fm =
+    merge R (set_frame r rr0 rr1 rr2 rr3 rr4 rr5 rr6 rr7 fm).
+Proof.
+  intros.
+  unfolds set_frame.
+  destruct fm.
+  eapply indoms_setRs_merge_eq2; eauto.
+Qed.
+
+Lemma setR_dom_eq2 :
+  forall R R' rn w,
+    dom_eq R R' ->
+    dom_eq R (set_R R' rn w).
+Proof.
+  intros.
+  unfold dom_eq in *.
+  simpljoin1.
+  split.
+  {
+    intros.
+    eapply H in H1.
+    clear - H1.
+    unfold indom in *.
+    simpljoin1.
+    unfold set_R.
+    unfold is_indom.
+    destruct (R' rn); eauto.
+    unfold RegMap.set.
+    destruct_rneq.
+  }
+  {
+    intros.
+    eapply H0.
+    clear - H1.
+    unfold indom in *.
+    simpljoin1.
+    unfolds set_R.
+    unfold is_indom in *.
+    destruct (R' rn) eqn:Heqe; eauto.
+    unfolds RegMap.set.
+    destruct_rneq_H.
+    subst.
+    inversion H; subst.
+    eauto.
+  }
+Qed.
+
+Lemma setframe_dom_eq :
+  forall R R' (rr0 rr1 rr2 rr3 rr4 rr5 rr6 rr7 : GenReg) fm,
+    dom_eq R R' ->
+    dom_eq R (set_frame R' rr0 rr1 rr2 rr3 rr4 rr5 rr6 rr7 fm).
+Proof.
+  intros.
+  unfold set_frame.
+  destruct fm.
+  simpls.
+  repeat (eapply setR_dom_eq2; eauto).
+Qed.
+
+Lemma set_win_merge1 :
+  forall (R1 R2 : RegFile) fm1 fm2 fm3,
+    indoms Fmr R1 ->
+    disjoint R1 R2 ->
+    set_window (merge R1 R2) fm1 fm2 fm3 = merge (set_window R1 fm1 fm2 fm3) R2.
+Proof.  
+  intros.
+  unfolds set_window.
+  rewrite fetch_some_set_frm_merge_eq; eauto.
+  rewrite fetch_some_set_frm_merge_eq; eauto.
+  rewrite fetch_some_set_frm_merge_eq; eauto.
+
+  do 2 eapply indoms_set_frm_still; eauto.
+  simpls.
+  simpljoin1.
+  repeat (split; eauto).
+
+  eapply indoms_set_frm_still.
+  simpls.
+  simpljoin1.
+  repeat (split; eauto).
+
+  simpls.
+  simpljoin1.
+  repeat (split; eauto).
+Qed.
+
+Lemma set_win_merge2 :
+  forall (R1 R2 : RegFile) fm1 fm2 fm3,
+    indoms Fmr R2 ->
+    disjoint R1 R2 ->
+    set_window (merge R1 R2) fm1 fm2 fm3 = merge R1 (set_window R2 fm1 fm2 fm3).
+Proof.
+  intros.
+  unfolds set_window.
+  rewrite fetch_some_set_frm_merge_eq2; eauto.
+  rewrite fetch_some_set_frm_merge_eq2; eauto.
+  rewrite fetch_some_set_frm_merge_eq2; eauto.
+  do 3 try eapply disjoint_setfrm_still2; eauto.
+
+  eapply disj_dom_eq_still; eauto.
+  eapply same_m_dom_eq; eauto.
+  repeat (eapply setframe_dom_eq; eauto).
+  eapply same_m_dom_eq; eauto.
+  
+  do 2 eapply indoms_set_frm_still; eauto.
+  simpl in H.
+  simpl.
+  simpljoin1.
+  repeat (split; eauto).
+
+  eapply disj_dom_eq_still; eauto.
+  eapply same_m_dom_eq; eauto.
+  repeat (eapply setframe_dom_eq; eauto).
+  eapply same_m_dom_eq; eauto.
+  eapply indoms_set_frm_still; eauto.
+  simpl in H.
+  simpljoin1.
+  simpl.
+  repeat (split; eauto).
+
+  simpls.
+  simpljoin1.
+  repeat (split; eauto).
+Qed.
+
+Lemma Reg_frm_upd :
+  forall M R R' F D (rr0 rr1 rr2 rr3 rr4 rr5 rr6 rr7 : GenReg) 
+    w0 w1 w2 w3 w4 w5 w6 w7 w0' w1' w2' w3' w4' w5' w6' w7',
+    (M, (R, F), D) |=
+                   rr0 |=> w0 ** rr1 |=> w1 ** rr2 |=> w2 ** rr3 |=> w3 **
+                   rr4 |=> w4 ** rr5 |=> w5 ** rr6 |=> w6 ** rr7 |=> w7 ->
+    (M, (R', F), D) |=
+                    rr0 |=> w0' ** rr1 |=> w1' ** rr2 |=> w2' ** rr3 |=> w3' **
+                    rr4 |=> w4' ** rr5 |=> w5' ** rr6 |=> w6' ** rr7 |=> w7' ->
+    R' = set_frame R rr0 rr1 rr2 rr3 rr4 rr5 rr6 rr7
+                   ([[w0', w1', w2', w3', w4', w5', w6', w7']]).
+Proof.
+  intros.
+
+  lets Hindom : regfrm_indoms H ___; eauto.
+  eapply Reg_upd with (w' := w0') in H.
+
+  eapply sep_star_lift in H.
+  eapply Reg_upd with (w' := w1') in H.
+  eapply sep_star_lift in H.
+   
+  eapply sep_star_assoc in H.
+  eapply sep_star_lift in H.
+  eapply Reg_upd with (w' := w2') in H.
+  eapply sep_star_lift in H.
+  eapply sep_star_assoc2 in H; eauto.
+
+  do 2 eapply sep_star_assoc in H.
+  eapply sep_star_lift in H.
+  eapply Reg_upd with (w' := w3') in H.
+  eapply sep_star_lift in H.
+  do 2 eapply sep_star_assoc2 in H; eauto.
+
+  do 3 eapply sep_star_assoc in H.
+  eapply sep_star_lift in H.
+  eapply Reg_upd with (w' := w4') in H.
+  eapply sep_star_lift in H.
+  do 3 eapply sep_star_assoc2 in H; eauto.
+
+  do 4 eapply sep_star_assoc in H.
+  eapply sep_star_lift in H.
+  eapply Reg_upd with (w' := w5') in H.
+  eapply sep_star_lift in H.
+  do 4 eapply sep_star_assoc2 in H; eauto.
+
+  do 5 eapply sep_star_assoc in H.
+  eapply sep_star_lift in H.
+  eapply Reg_upd with (w' := w6') in H.
+  eapply sep_star_lift in H.
+  do 5 eapply sep_star_assoc2 in H; eauto.
+
+  do 6 eapply sep_star_assoc in H.
+  eapply sep_star_sym in H.
+  eapply Reg_upd with (w' := w7') in H.
+  eapply sep_star_sym in H.
+  do 6 eapply sep_star_assoc2 in H.
+
+  lets Ht : Reg_frm_precise ___; eauto.
+  unfolds precise_asrt.  
+  eapply Ht in H; eauto.
+  simpljoin1.
+  subst.
+  unfold set_frame.
+  unfold set_Rs.
+
+  simpl in Hindom.
+  simpljoin1.
+  do 8 (rewrite indom_setR_eq_RegMap_set; eauto;
+        try (repeat eapply indom_regset_still; eauto)).
+Qed.
+
+Lemma OutRegs_setframe :
+  forall M R R' F D fm fm',
+    (M, (R, F), D) |= OutRegs fm ->
+    (M, (R', F), D) |= OutRegs fm' ->
+    R' = set_frame R r8 r9 r10 r11 r12 r13 r14 r15 fm'.
+Proof.
+  intros.
+  unfolds OutRegs.
+  destruct fm, fm'.    
+  eapply Reg_frm_upd; eauto.
+Qed.
+
+Lemma LocalRegs_setframe :
+  forall M R R' F D fm fm',
+    (M, (R, F), D) |= LocalRegs fm ->
+    (M, (R', F), D) |= LocalRegs fm' ->
+    R' = set_frame R r16 r17 r18 r19 r20 r21 r22 r23 fm'.
+Proof.
+  intros.
+  unfolds LocalRegs.
+  destruct fm, fm'.    
+  eapply Reg_frm_upd; eauto.
+Qed.
+
+Lemma InRegs_setframe :
+  forall M R R' F D fm fm',
+    (M, (R, F), D) |= InRegs fm ->
+    (M, (R', F), D) |= InRegs fm' ->
+    R' = set_frame R r24 r25 r26 r27 r28 r29 r30 r31 fm'.
+Proof.
+  intros.
+  unfolds InRegs.
+  destruct fm, fm'.    
+  eapply Reg_frm_upd; eauto.
+Qed.
+
+Lemma set_window_res :
+  forall M R R' F D fm1 fm2 fm3 fm1' fm2' fm3',
+    (M, (R, F), D) |= Regs fm1 fm2 fm3 ->
+    (M, (R', F), D) |= Regs fm1' fm2' fm3' ->
+    set_window R fm1' fm2' fm3' = R'.
+Proof.
+  intros. 
+  unfold set_window.
+
+  unfolds Regs.
+  eapply sep_star_split in H.
+  simpljoin1.
+  renames x to s1, x0 to s.
+  eapply sep_star_split in H1.
+  simpljoin1.
+  renames x to s2, x0 to s3.
+
+  eapply sep_star_split in H0.
+  simpljoin1.
+  renames x to s1', x0 to s'.
+  eapply sep_star_split in H5.
+  simpljoin1.
+  renames x to s2', x0 to s3'.
+
+  destruct_state s1.
+  destruct_state s2.
+  destruct_state s3.
+  destruct_state s.
+  simpl in H2, H4.
+  simpljoin1.
+
+  destruct_state s1'.
+  destruct_state s2'.
+  destruct_state s3'.
+  destruct_state s'.
+  simpl in H8, H6.
+  simpljoin1.
+  
+  rewrite fetch_some_set_frm_merge_eq.
+  rewrite fetch_some_set_frm_merge_eq2.
+
+  assert (set_frame (merge r0 r1) r16 r17 r18 r19 r20 r21 r22 r23 fm2' =
+          merge (set_frame r0 r16 r17 r18 r19 r20 r21 r22 r23 fm2') r1).
+  {
+    rewrite fetch_some_set_frm_merge_eq; eauto.
+    eapply LocalRegs_indoms; eauto.
+  }
+  rewrite H11.
+
+  rewrite fetch_some_set_frm_merge_eq2.
+  rewrite fetch_some_set_frm_merge_eq2.
+  
+  erewrite <- OutRegs_setframe with (R' := r2); eauto.
+  erewrite <- InRegs_setframe with (R' := r4); eauto. 
+  erewrite <- LocalRegs_setframe with (R' := r3); eauto.
+
+  admit.
+  admit.
+  admit.
+  
+  eapply disjoint_setfrm_still; eauto.
+  eapply InRegs_indoms; eauto.
+
+  eapply disjoint_setfrm_still; eauto.
+  eapply disj_sep_merge_still; eauto.
+  eapply disjoint_setfrm_still2; eauto.
+  eapply disj_merge_disj_sep1 in H2; eauto.
+  eapply disj_merge_disj_sep2 in H2; eauto.
+
+  eapply indoms_merge_still2; eauto.
+  eapply InRegs_indoms; eauto.
+
+  eapply disjoint_setfrm_still; eauto.
+
+  eapply indoms_merge_still1; eauto.
+  eapply LocalRegs_indoms; eauto.
+
+  eapply OutRegs_indoms; eauto.
+Qed.
+
+Lemma Regs_frm_free :
+  forall M R F F' D fm1 fm2 fm3,
+    (M, (R, F), D) |= Regs fm1 fm2 fm3 ->
+    (M, (R, F'), D) |= Regs fm1 fm2 fm3.
+Proof.
+Admitted.
+(*
+  intros.
+  unfolds Regs.
+  eapply sep_star_split in H; eauto.
+  simpljoin1.
+  eapply sep_star_split in H0; eauto.
+  simpljoin1.
+  destruct_state x.
+  destruct_state x1.
+  destruct_state x2.
+
+  simpl in H1, H3.
+  destruct_state x0.
+  simpljoin1.
+
+  eapply disj_sep_star_merge; eauto.
+  eapply OutRegs_frm_free; eauto.
+
+  eapply disj_sep_star_merge; eauto.
+  eapply LocalRegs_frm_free; eauto.
+  eapply InRegs_frm_free; eauto.
+Qed.*)
+
+Lemma Regs_indom_Fmr :
+  forall M R F D fm1 fm2 fm3,
+    (M, (R, F), D) |= Regs fm1 fm2 fm3 ->
+    indoms Fmr R.
+Proof.
+  intros.
+  unfolds Regs.
+  sep_star_split_tac.
+  simpl in H2, H3.
+  simpljoin1.
+(*
+  eapply OutRegs_indoms in H; eauto.
+  eapply LocalRegs_indoms in H0; eauto.
+  eapply InRegs_indoms in H1; eauto.
+
+  simpls.
+  simpljoin1.
+
+  repeat
+    (
+      split;
+      [
+        try solve [eapply indom_merge_still; eauto];
+        try solve [eapply indom_merge_still2; eapply indom_merge_still; eauto];
+        try solve [eapply indom_merge_still2; eapply indom_merge_still2; eauto] |
+        idtac
+      ]
+    ).
+  eauto.
+Qed.*)
+Admitted.
   
 (*+ Soundness Proof of instruction +*)
 
@@ -2265,11 +3239,114 @@ Proof.
     eapply fetch_disj_merge_still2; eauto.
     eapply fetch_disj_merge_still1; eauto.
     eapply Regs_fetch; eauto.
-    
-    >>>>>>>>>>>>>>>>>>>>>>>>>>>
   }
-  
+  {
+    eapply indom_merge_still2; eauto.
+    eapply indom_dom_eq_subst with (m := (r' ⊎ (r1' ⊎ r3))).
+    rewrite H28.
+    eapply indom_merge_still; eauto.
+    eapply regset_l_l_indom; eauto.
+    eapply dom_eq_merge_still; eauto.
+    eapply dom_eq_sym; eauto.
+    eapply dom_eq_merge_still; eauto.
+    eapply dom_eq_sym; eauto.
+    eapply same_m_dom_eq; eauto.
+  }
+  {
+    instantiate (1 := v1).
+    clear - H H4 Ht.
+    eapply H in Ht; eauto.
+    simpl in Ht.
+    simpljoin1.
+    eapply get_vl_merge_still2; eauto.
+  }
+  {
+    instantiate (1 := v2).
+    clear - H H4 Ht.
+    eapply H in Ht; eauto.
+    simpl in Ht.
+    simpljoin1.
+    eapply eval_opexp_merge_still2; eauto.
+  }
+  { 
+    rewrite set_win_merge2; eauto.
+    rewrite set_win_merge2; eauto.
+    rewrite set_win_merge1; eauto.
+    erewrite set_window_res with (R' := r1'); eauto.
 
+    unfold set_Rs.
+    rewrite indom_setR_merge_eq2; eauto. 
+    assert (set_R (r ⊎ (r1' ⊎ r3)) cwp (pre_cwp id) =
+            (set_R r cwp (pre_cwp id)) ⊎ (r1' ⊎ r3)).
+    {
+      rewrite indom_setR_merge_eq1; eauto.
+      clear - H6.
+      simpls.
+      unfolds regSt.
+      simpls.
+      simpljoin1.
+      eapply regset_l_l_indom; eauto.
+    }
+    rewrite H17; eauto.
+    assert (set_R r cwp (pre_cwp id) = r').
+    {
+      clear - H6 H13.
+      simpls.
+      unfolds regSt.
+      simpls.
+      simpljoin1.
+      rewrite indom_setR_eq_RegMap_set; eauto.
+      rewrite regset_twice; eauto.
+      eapply regset_l_l_indom; eauto.
+    }
+    rewrite H20.
+    rewrite H28.
+    rewrite indom_setR_merge_eq2; eauto.
+    rewrite indom_setR_merge_eq1; eauto.
+    rewrite indom_setR_eq_RegMap_set; eauto.
+    rewrite regset_twice; eauto.
+    eapply regset_l_l_indom; eauto.
+    eapply regset_l_l_indom; eauto.
+
+    clear.
+    unfold indom.
+    intro.
+    simpljoin1.
+    unfolds RegMap.set.
+    destruct_rneq_H.
+
+    rewrite <- H28.
+    eapply disj_dom_eq_still with (m2 := (r ⊎ (r1 ⊎ r3))); eauto.
+    eapply same_m_dom_eq; eauto.
+    eapply dom_eq_merge_still; eauto.
+    eapply dom_eq_merge_still; eauto.
+    eapply same_m_dom_eq; eauto.
+
+    clear.
+    unfold indom.
+    intro.
+    simpljoin1.
+    unfolds RegMap.set.
+    destruct_rneq_H.
+
+    eapply disj_dom_eq_still with (m2 := (r ⊎ (r1 ⊎ r3))); eauto.
+    eapply same_m_dom_eq; eauto.
+    eapply dom_eq_merge_still; eauto.
+    eapply same_m_dom_eq; eauto.
+    eapply dom_eq_merge_still; eauto.
+    eapply same_m_dom_eq; eauto.
+
+    clear - H15.
+    eapply Regs_frm_free; eauto.
+    eapply Regs_indom_Fmr; eauto.
+    eapply indoms_merge_still1; eauto.
+    eapply Regs_indom_Fmr; eauto.
+    eapply indoms_merge_still2; eauto.
+    eapply indoms_merge_still1; eauto.
+    eapply Regs_indom_Fmr; eauto.
+  }
+Qed.
+  
 Lemma resotre_rule_sound :
   forall p q (rs rd : GenReg) v1 v2 v v' id id' F fm1 fm2 fmo fml fmi p1 oexp,
     p ==> Or rs ==ₑ v1 //\\ oexp ==ₑ v2 ->
@@ -2278,7 +3355,279 @@ Lemma resotre_rule_sound :
     {|id', F ++ [fmo; fml]|} ** Regs fmi fm1 fm2 ** p1 ==> rd |=> v' ** q ->
     ins_sound (Rwim |=> v ** p) (Rwim |=> v ** rd |=> v1 +ᵢ v2 ** q) (restore rs oexp rd).
 Proof.
-  Admitted.
+  intros.
+  unfolds ins_sound.
+  intros.
+  destruct_state s.
+  simpl in H4.
+  simpljoin1.
+  destruct_state x.
+  destruct_state x0.
+  simpl in H4.
+  simpljoin1.
+
+  lets Ht : H6.
+  lets Ht1 : H6.
+  eapply H0 in H6.
+
+  eapply sep_star_split in H6.
+  simpljoin1.
+  destruct_state x.
+  destruct_state x0.
+ 
+  simpl in H8.
+  simpljoin1.
+  eapply sep_star_split in H7; eauto.
+  simpljoin1.
+  destruct_state x.
+  destruct_state x0.
+  simpl in H11.
+  simpljoin1.
+
+  assert (f1 = fm1 :: fm2 :: F).
+  { 
+    clear - H6.
+    simpl in H6.
+    simpljoin1; eauto.
+  }
+
+  subst.  
+  lets Hf : H6.
+  eapply frame_asrt_upd with (id' := post_cwp id) (F' := F ++ [fmo; fml]) in Hf; eauto.
+  simpljoin1.
+  rename x into r'.
+
+  lets Hreg : H7. 
+  eapply Regs_asrt_upd with
+  (F' := F ++ [fmo; fml]) (fm1' := fmi) (fm2' := fm1) (fm3' := fm2) in Hreg.
+ 
+  simpljoin1.
+  rename x into r1'.
+  eapply asrt_FrmFree_changefrm_stable with (F' := F ++ [fmo; fml]) in H10; eauto.
+
+  Focus 2.
+  clear - H6 H9. 
+  eapply disj_merge_disj_sep2 in H9.
+  intro.
+  simpl in H6.
+  simpljoin1.
+  unfolds regSt.
+  simpls.
+  simpljoin1.
+  unfold disjoint in *.
+  specialize (H9 cwp).
+  unfolds RegMap.set. 
+  destruct_rneq_H.
+  unfold indom in *; simpljoin1.
+  rewrite H in H9; tryfalse.
+
+  assert
+    (Htt : 
+      ((merge m (merge m1 m3)), (merge r' (merge r1' r3), F ++ [fmo; fml]), d1) |=
+      {|post_cwp id, F ++ [fmo; fml]|} ** Regs fmi fm1 fm2 ** p1
+    ).
+  {  
+    eapply disj_sep_star_merge; eauto.
+    eapply disj_sep_star_merge; eauto. 
+    eapply disj_dom_eq_still.
+    2 : eauto. 
+    eauto.
+    eapply same_m_dom_eq.
+    
+    eauto.
+    eapply disj_sep_merge_still; eauto.
+    eapply disj_merge_disj_sep1 in H9; eauto.
+    eapply disj_dom_eq_still; eauto.
+    eapply disj_merge_disj_sep2 in H9; eauto.
+    eapply disj_dom_eq_still; eauto.
+    eapply same_m_dom_eq; eauto.
+  }
+
+  unfolds regSt.
+  simpl in H5.
+  simpljoin1.
+  eapply H3 in Htt.
+
+  simpl in Htt.
+  simpljoin1.
+  destruct_state x.
+  destruct_state x0.
+  unfolds regSt.
+  simpl in H5, H17.
+  simpljoin1.
+  
+  eexists.
+  split.
+  Focus 2.
+  simpl.
+ 
+  exists (empM, (RegMap.set Rwim (Some v) empR, F ++ [fmo; fml]), d0).
+  eexists.
+  split.
+
+  Focus 2.
+  split.
+  unfold regSt.
+  simpl.
+  repeat (split; eauto).
+ 
+  exists (empM, (RegMap.set rd (Some (v1 +ᵢ v2)) empR, F ++ [fmo; fml]), d0).
+  eexists.
+  split.
+  Focus 2.
+  split; eauto.
+  unfold regSt.
+  simpl.
+  split; eauto.
+   
+  simpl.
+  repeat (split; eauto).
+  eapply RegSet_same_addr_disj_stable; eauto.
+ 
+  simpl.
+  repeat (split; eauto).
+  eapply disj_dom_eq_still with (m1 := RegMap.set Rwim (Some v) empR)
+                                  (m2 := r ⊎ (r1 ⊎ r3)); eauto.
+  eapply dom_eq_memset_same_addr_stable; eauto.
+  eapply dom_eq_emp; eauto.
+  eapply dom_eq_trans with (m2 := merge r' (merge r1' r3)).
+  repeat (eapply dom_eq_merge_still; eauto).
+  eapply same_m_dom_eq; eauto.
+  rewrite H28; eauto.
+  eapply dom_eq_merge_some_addr_stable; eauto.
+  eapply same_m_dom_eq; eauto.
+
+  rewrite H27. 
+  eapply RRestore; eauto.
+  {
+    eapply get_vl_merge_still2; eauto.
+    eapply get_vl_merge_still; eauto.
+    clear - H6.
+    simpls.
+    unfolds regSt.
+    simpls.
+    simpljoin1.
+    unfold RegMap.set.
+    destruct_rneq.
+  }
+  {
+    eapply get_vl_merge_still; eauto.
+    unfold RegMap.set.
+    destruct_rneq.
+  }
+  {
+    instantiate (1 := fmi).
+    eapply fetch_disj_merge_still2; eauto.
+    eapply fetch_disj_merge_still2; eauto.
+    eapply fetch_disj_merge_still1; eauto.
+    eapply Regs_fetch; eauto.
+  }
+  {
+    eapply indom_merge_still2; eauto.
+    eapply indom_dom_eq_subst with (m := (r' ⊎ (r1' ⊎ r3))).
+    rewrite H28.
+    eapply indom_merge_still; eauto.
+    eapply regset_l_l_indom; eauto.
+    eapply dom_eq_merge_still; eauto.
+    eapply dom_eq_sym; eauto.
+    eapply dom_eq_merge_still; eauto.
+    eapply dom_eq_sym; eauto.
+    eapply same_m_dom_eq; eauto.
+  }
+  {
+    instantiate (1 := v1).
+    clear - H H4 Ht.
+    eapply H in Ht; eauto.
+    simpl in Ht.
+    simpljoin1.
+    eapply get_vl_merge_still2; eauto.
+  }
+  {
+    instantiate (1 := v2).
+    clear - H H4 Ht.
+    eapply H in Ht; eauto.
+    simpl in Ht.
+    simpljoin1.
+    eapply eval_opexp_merge_still2; eauto.
+  }
+  { 
+    rewrite set_win_merge2; eauto.
+    rewrite set_win_merge2; eauto.
+    rewrite set_win_merge1; eauto.
+    erewrite set_window_res with (R' := r1'); eauto.
+
+    unfold set_Rs.
+    rewrite indom_setR_merge_eq2; eauto. 
+    assert (set_R (r ⊎ (r1' ⊎ r3)) cwp (post_cwp id) =
+            (set_R r cwp (post_cwp id)) ⊎ (r1' ⊎ r3)).
+    {
+      rewrite indom_setR_merge_eq1; eauto.
+      clear - H6.
+      simpls.
+      unfolds regSt.
+      simpls.
+      simpljoin1.
+      eapply regset_l_l_indom; eauto.
+    }
+    rewrite H17; eauto.
+    assert (set_R r cwp (post_cwp id) = r').
+    {
+      clear - H6 H13.
+      simpls.
+      unfolds regSt.
+      simpls.
+      simpljoin1.
+      rewrite indom_setR_eq_RegMap_set; eauto.
+      rewrite regset_twice; eauto.
+      eapply regset_l_l_indom; eauto.
+    }
+    rewrite H20.
+    rewrite H28.
+    rewrite indom_setR_merge_eq2; eauto.
+    rewrite indom_setR_merge_eq1; eauto.
+    rewrite indom_setR_eq_RegMap_set; eauto.
+    rewrite regset_twice; eauto.
+    eapply regset_l_l_indom; eauto.
+    eapply regset_l_l_indom; eauto.
+
+    clear.
+    unfold indom.
+    intro.
+    simpljoin1.
+    unfolds RegMap.set.
+    destruct_rneq_H.
+
+    rewrite <- H28.
+    eapply disj_dom_eq_still with (m2 := (r ⊎ (r1 ⊎ r3))); eauto.
+    eapply same_m_dom_eq; eauto.
+    eapply dom_eq_merge_still; eauto.
+    eapply dom_eq_merge_still; eauto.
+    eapply same_m_dom_eq; eauto.
+
+    clear.
+    unfold indom.
+    intro.
+    simpljoin1.
+    unfolds RegMap.set.
+    destruct_rneq_H.
+
+    eapply disj_dom_eq_still with (m2 := (r ⊎ (r1 ⊎ r3))); eauto.
+    eapply same_m_dom_eq; eauto.
+    eapply dom_eq_merge_still; eauto.
+    eapply same_m_dom_eq; eauto.
+    eapply dom_eq_merge_still; eauto.
+    eapply same_m_dom_eq; eauto.
+
+    clear - H15.
+    eapply Regs_frm_free; eauto.
+    eapply Regs_indom_Fmr; eauto.
+    eapply indoms_merge_still1; eauto.
+    eapply Regs_indom_Fmr; eauto.
+    eapply indoms_merge_still2; eauto.
+    eapply indoms_merge_still1; eauto.
+    eapply Regs_indom_Fmr; eauto.
+  }
+Qed.
 
 Lemma conj_ins_sound : forall p1 p2 q1 q2 i,
     ins_sound p1 q1 i -> ins_sound p2 q2 i -> ins_sound (p1 //\\ p2) (q1 //\\ q2) i.
